theories/examples/finelt/types.v
@@ -598,3 +598,4 @@ Proof.
       inversion A1. subst r. done.
 Qed.
 
+
